# Expression #1
#### Expression
```
10
```
#### Description
Evaluate the primitive expression $10$.
#### Result
```
10
```
# Expression #2
#### Expression
```
(+ 5 3 4)
```
#### Description
Calculate $5 + 3 + 4$
#### Result
```
12
```
# Expression #3
#### Expression
```
(- 9 1)
```
#### Description
Calculate $9 - 1$
#### Result
```
8
```
# Expression #4
#### Expression
```
(/ 6 2)
```
#### Description
Calculate $6 / 2$
#### Result
```
3
```
# Expression #5
#### Expression
```
(+ (* 2 4) (- 4 6))
```
#### Description
Calculate $(2 * 4) + (4 - 6)$
#### Result
```
6
```
# Expression #6
#### Expression
```
(define a 3)
```
#### Description
Define a new variable called $a$ with the value of $3$.
#### Result
```
```
# Expression #7
#### Expression
```
(define b (+ a 1))
```
#### Description
Define a new variable called $b$ with the value of $(a + 1)$.
(Where $a = 3$)
#### Result
```
```
# Expression #8
#### Expression
```
(+ a b (* a b))
```
#### Description
Calculate $a + b + (a * b)$
(Where $a = 3$ and $b = 4$)
$$
\begin{align}
a + b + (a * b) &= a + b + (3 * 4)\\
&= a + b + 12\\
&= 3 + 4 + 12\\
&= 19
\end{align}
$$
#### Result
```
19
```
# Expression #9
#### Expression
```
(= a b)
```
#### Description
Check if the value of $a$ is equal to the value of $b$
(Where $a = 3$ and $b = 4$)
#### Result
```
#f
```
# Expression #10
#### Expression
```
(if (and (> b a) (< b (* a b)))
    b
    a)
```
#### Description
Evaluate a conditional expression :
* If $b > a$ and $b < (a * b)$, the result is $b$.
* Otherwise, the result is $a$.
(Where $a = 3$ and $b = 4$)
#### Result
```
4
```
# Expression #11
#### Expression
```
(cond (( = a 4) 6)
      (( = b 4) (+ 6 7 a))
      (else 25)) 
```
#### Description
Evaluate a conditional expression :
* If $a = 4$, the result is $6$.
* If $b = 4$, the result is $6 + 7 + a$
* Otherwise, the result is $25$
(Where $a = 3$ and $b = 4$)
#### Result
```
16
```
# Expression #12
#### Expression
```
(+ 2 (if (> b a) b a))
```
#### Description
If $b$ is greater than $a$, the result is $b$.
If not, the result is $a$.
(Where $a = 3$ and $b = 4$)
#### Result
```
6
```
# Expression #13
#### Expression
```
(* (cond (( > a b) a)
         (( < a b) b)
         (else -1))
   (+ a 1))
```
#### Description
First, evaluate ```cond``` expression
* If $a > b$, the result is $a$.
* If $a < b$, the result is b.
* Otherwise, the result is $-1$.
Then, multiply this result by $a + 1$.
(Where $a = 3$ and $b = 4$)
#### Result
```
16
```